omg this is terrible

src/Dmajor.v
@@ -255,15 +255,7 @@ Inductive step: state -> trace -> state -> Prop :=
 
 End RELSEM.
 
-
-Inductive initial_state (p: program): state -> Prop :=
-  | initial_state_intro: forall b f m0,
-      let ge := Genv.globalenv p in
-      Genv.init_mem p = Some m0 ->
-      Genv.find_symbol ge p.(prog_main) = Some b ->
-      Genv.find_funct_ptr ge b = Some (Internal f) ->
-      funsig f = signature_main ->
-      initial_state p (Callstate f nil Kstop m0).
+Inductive is_callstate (p : program) : value -> value -> state -> Prop := .
 
 (** A final state is a [Returnstate] with an empty continuation. *)
 Inductive final_state (p : program): state -> value -> Prop :=
@@ -275,7 +267,7 @@ Inductive final_state (p : program): state -> value -> Prop :=
 (** The corresponding small-step semantics. *)
 
 Definition semantics (p: program) :=
-  Semantics step (initial_state p) (final_state p) (Genv.globalenv p).
+  Semantics step (is_callstate p) (final_state p) (Genv.globalenv p).
 
 (** This semantics is receptive to changes in events. *)
 
