src/FlatIntTagComp.v
@@ -485,7 +485,7 @@ Section Preservation.
   Proof.
     eapply Semantics.forward_simulation_step with (match_states := I).
     - inversion 1. (* TODO - replace with callstate matching *)
-    - intros0 II Afinal. invc Afinal. invc II. on >I_cont, invc. constructor.
+    - intros0 II Afinal. invc Afinal. invc II. on >I_cont, invc. eexists; split. constructor. reflexivity.
     - intros0 Astep. intros0 II.
       eapply I_sim; eauto.
       destruct prog, tprog. eapply compile_cu_I_env; eauto.
